src/ASN1/ASN1.Spec.Choice.fst
@@ -1,4 +1,3 @@
-
 module ASN1.Spec.Choice
 
 open ASN1.Base
@@ -12,12 +11,6 @@ module Math = FStar.Math.Lib
 module List = FStar.List.Tot
 
 (*
-// Now defined in Base
-// Mention Shadowing
-
-let make_gen_choice_type (#key : eqtype) (lc : list (key & Type)) = (id : key) & (idlookup_t id lc)
-
-*)
 
 let sanitify_parser_kind (k : parser_kind)
 : Pure parser_kind
@@ -44,6 +37,8 @@ let rec make_gen_choice_kind
     sanitify_parser_kind k
   | h :: t -> glb (Mkgenparser?.k h) (make_gen_choice_kind t)
 
+*)
+
 let tag_of_gen_choice_type (#key : eqtype) (lc : list (key & Type)) : make_gen_choice_type lc -> Tot key = dfst
 
 let extract_types (#t : eqtype) (lc : list (t & gen_parser)) =
@@ -60,8 +55,7 @@ let rec make_gen_choice_payload_parser
   (#t : eqtype)
   (lc : list (t & gen_parser) {Cons? lc})
 //  (pf : List.noRepeats (List.map fst lc))
-  : Tot (id : t -> parser 
-                  (make_gen_choice_kind (List.map snd lc))
+  : Tot (id : t -> asn1_strong_parser 
                   (refine_with_tag (project_tags lc) id))
 = fun id ->
   match lc with
@@ -69,20 +63,19 @@ let rec make_gen_choice_payload_parser
     let (id', gp) = hd in
     if (id = id') then
       let p = (Mkgenparser?.p gp) in 
-      let p' = parse_synth p (attach_tag lc id) in
-      (weaken (make_gen_choice_kind (List.map snd lc)) p')
+      parse_synth p (attach_tag lc id)
     else      
       (match tl with
-      | nil -> fail_parser (make_gen_choice_kind (List.map snd lc)) (refine_with_tag (project_tags lc) id)
+      | nil -> fail_parser asn1_strong_parser_kind (refine_with_tag (project_tags lc) id)
       | _ -> make_gen_choice_payload_parser tl id)
-    
+
 let make_gen_choice_parser
   (#t : eqtype)
   (#k : parser_kind)
   (p : parser k t)
   (lc : list (t & gen_parser) {Cons? lc})
   //(pf : List.noRepeats (List.map fst lc))
-  : parser (and_then_kind k (make_gen_choice_kind (List.map snd lc))) (make_gen_choice_type (extract_types lc))
+  : parser (and_then_kind k asn1_strong_parser_kind) (make_gen_choice_type (extract_types lc))
 = parse_tagged_union p (tag_of_gen_choice_type (extract_types lc)) (make_gen_choice_payload_parser lc)
 
 let make_asn1_choice_parser
@@ -92,7 +85,32 @@ let make_asn1_choice_parser
   (k : asn1_k s)
   (lp : list (asn1_id_t & gen_parser) {Cons? lp})
   : 
-  Pure (parser (and_then_kind parse_asn1_identifier_u21_kind (make_gen_choice_kind (List.map snd lp))) (asn1_t k))
+  Pure (asn1_strong_parser (asn1_t k))
   (requires (s == Set.as_set (List.map fst lc)) /\ (k == ASN1_CHOICE_ILC lc pf) /\ (asn1_lc_t lc == extract_types lp))
   (ensures fun _ -> True)
-= make_gen_choice_parser parse_asn1_identifier_u21 lp
+= weaken asn1_strong_parser_kind (make_gen_choice_parser parse_asn1_identifier_u21 lp)
+
+let make_asn1_choice_parser_twin
+  (lc : list (asn1_id_t * asn1_content_k) {Cons? lc})
+  (pf : ((Cons? lc) /\ List.noRepeats (List.map fst lc)))
+  (#s : _)
+  (k : asn1_k s)
+  (lp : list (asn1_id_t & gen_parser) {Cons? lp})
+  (id' : asn1_id_t)
+  : 
+  Pure (asn1_strong_parser (asn1_t k))
+  (requires (s == Set.as_set (List.map fst lc)) /\ (k == ASN1_CHOICE_ILC lc pf) /\ (asn1_lc_t lc == extract_types lp))
+  (ensures fun _ -> True)
+= parse_tagged_union_payload (project_tags lp) (make_gen_choice_payload_parser lp) id'
+
+let make_asn1_choice_parser_twin_cases_injective
+  (lc : list (asn1_id_t * asn1_content_k) {Cons? lc})
+  (pf : ((Cons? lc) /\ List.noRepeats (List.map fst lc)))
+  (#s : _)
+  (k : asn1_k s)
+  (lp : list (asn1_id_t & gen_parser) {Cons? lp})
+  : 
+  Lemma 
+  (requires (s == Set.as_set (List.map fst lc)) /\ (k == ASN1_CHOICE_ILC lc pf) /\ (asn1_lc_t lc == extract_types lp))
+  (ensures and_then_cases_injective (make_asn1_choice_parser_twin lc pf k lp))
+= parse_tagged_union_payload_and_then_cases_injective (project_tags lp) (make_gen_choice_payload_parser lp)
